libcrux-iot/sha3/proofs/lean/LibcruxIotSha3/Extraction/Specs.lean
@@ -26,7 +26,7 @@ namespace libcrux_iot_sha3
 
 
 /-- [libcrux_iot_sha3::hash::pre]:
-    Source: 'sha3/src/lib.rs', lines 145:16-145:102 -/
+    Source: 'sha3/src/lib.rs', lines 150:16-150:102 -/
 @[reducible]
 def hash.pre
   (LEN : Std.Usize) (algorithm : Algorithm) (payload : Slice Std.U8) :
@@ -48,7 +48,7 @@ def hash.spec (LEN : Std.Usize) (algorithm : Algorithm)
 
 
 /-- [libcrux_iot_sha3::sha224::pre]:
-    Source: 'sha3/src/lib.rs', lines 178:16-178:69 -/
+    Source: 'sha3/src/lib.rs', lines 183:16-183:69 -/
 @[reducible]
 def sha224.pre (payload : Slice Std.U8) : RustM Bool := do
   let i ← core.slice.Slice.len payload
@@ -63,7 +63,7 @@ def sha224.spec (payload : Slice Std.U8) : Prop :=
 
 
 /-- [libcrux_iot_sha3::sha224_ema::pre]:
-    Source: 'sha3/src/lib.rs', lines 197:16-197:109 -/
+    Source: 'sha3/src/lib.rs', lines 202:16-202:109 -/
 @[reducible]
 def sha224_ema.pre
   (digest : Slice Std.U8) (payload : Slice Std.U8) : RustM Bool := do
@@ -75,7 +75,7 @@ def sha224_ema.pre
   else ok false
 
 /-- [libcrux_iot_sha3::sha224_ema::post]:
-    Source: 'sha3/src/lib.rs', lines 201:0-201:84 -/
+    Source: 'sha3/src/lib.rs', lines 206:0-206:84 -/
 @[reducible]
 def sha224_ema.post
   (digest : Slice Std.U8) (payload : Slice Std.U8)
@@ -93,7 +93,7 @@ def sha224_ema.spec (digest : Slice Std.U8) (payload : Slice Std.U8) : Prop :=
 
 
 /-- [libcrux_iot_sha3::sha256::pre]:
-    Source: 'sha3/src/lib.rs', lines 215:16-215:69 -/
+    Source: 'sha3/src/lib.rs', lines 220:16-220:69 -/
 @[reducible]
 def sha256.pre (payload : Slice Std.U8) : RustM Bool := do
   let i ← core.slice.Slice.len payload
@@ -108,7 +108,7 @@ def sha256.spec (payload : Slice Std.U8) : Prop :=
 
 
 /-- [libcrux_iot_sha3::sha256_ema::pre]:
-    Source: 'sha3/src/lib.rs', lines 234:16-234:109 -/
+    Source: 'sha3/src/lib.rs', lines 239:16-239:109 -/
 @[reducible]
 def sha256_ema.pre
   (digest : Slice Std.U8) (payload : Slice Std.U8) : RustM Bool := do
@@ -120,7 +120,7 @@ def sha256_ema.pre
   else ok false
 
 /-- [libcrux_iot_sha3::sha256_ema::post]:
-    Source: 'sha3/src/lib.rs', lines 238:0-238:84 -/
+    Source: 'sha3/src/lib.rs', lines 241:0-243:67 -/
 @[reducible]
 def sha256_ema.post
   (digest : Slice Std.U8) (payload : Slice Std.U8)
@@ -128,7 +128,23 @@ def sha256_ema.post
   RustM Bool
   := do
   let i ← core.slice.Slice.len digest_future
-  ok (i = SHA3_256_DIGEST_SIZE)
+  if i = SHA3_256_DIGEST_SIZE
+  then
+    let s ←
+      libcrux_secrets.SharedASlice.Insts.Libcrux_secretsTraitsDeclassifyRefSharedASlice.declassify_ref
+        libcrux_secrets.U8.Insts.Libcrux_secretsTraitsScalar digest_future
+    let s1 ←
+      libcrux_secrets.SharedASlice.Insts.Libcrux_secretsTraitsDeclassifyRefSharedASlice.declassify_ref
+        libcrux_secrets.U8.Insts.Libcrux_secretsTraitsScalar payload
+    let a ← hacspec_sha3.sha3.sha3_256 s1
+    let s2 ←
+      core.Array.Insts.CoreOpsIndexIndex.index
+        (core.Slice.Insts.CoreOpsIndexIndex
+        (core.ops.range.RangeFull.Insts.CoreSliceIndexSliceIndexSliceSlice
+        Std.U8)) a ()
+    core.Slice.Insts.CoreCmpPartialEqSlice.eq core.U8.Insts.CoreCmpPartialEqU8
+      s s2
+  else ok false
 
 def sha256_ema.spec (digest : Slice Std.U8) (payload : Slice Std.U8) : Prop :=
   (sha256_ema.pre digest payload).holds →
@@ -138,7 +154,7 @@ def sha256_ema.spec (digest : Slice Std.U8) (payload : Slice Std.U8) : Prop :=
 
 
 /-- [libcrux_iot_sha3::sha384::pre]:
-    Source: 'sha3/src/lib.rs', lines 252:16-252:69 -/
+    Source: 'sha3/src/lib.rs', lines 257:16-257:69 -/
 @[reducible]
 def sha384.pre (payload : Slice Std.U8) : RustM Bool := do
   let i ← core.slice.Slice.len payload
@@ -153,7 +169,7 @@ def sha384.spec (payload : Slice Std.U8) : Prop :=
 
 
 /-- [libcrux_iot_sha3::sha384_ema::pre]:
-    Source: 'sha3/src/lib.rs', lines 271:16-271:109 -/
+    Source: 'sha3/src/lib.rs', lines 276:16-276:109 -/
 @[reducible]
 def sha384_ema.pre
   (digest : Slice Std.U8) (payload : Slice Std.U8) : RustM Bool := do
@@ -165,7 +181,7 @@ def sha384_ema.pre
   else ok false
 
 /-- [libcrux_iot_sha3::sha384_ema::post]:
-    Source: 'sha3/src/lib.rs', lines 275:0-275:84 -/
+    Source: 'sha3/src/lib.rs', lines 280:0-280:84 -/
 @[reducible]
 def sha384_ema.post
   (digest : Slice Std.U8) (payload : Slice Std.U8)
@@ -183,7 +199,7 @@ def sha384_ema.spec (digest : Slice Std.U8) (payload : Slice Std.U8) : Prop :=
 
 
 /-- [libcrux_iot_sha3::sha512::pre]:
-    Source: 'sha3/src/lib.rs', lines 289:16-289:69 -/
+    Source: 'sha3/src/lib.rs', lines 294:16-294:69 -/
 @[reducible]
 def sha512.pre (payload : Slice Std.U8) : RustM Bool := do
   let i ← core.slice.Slice.len payload
@@ -198,7 +214,7 @@ def sha512.spec (payload : Slice Std.U8) : Prop :=
 
 
 /-- [libcrux_iot_sha3::sha512_ema::pre]:
-    Source: 'sha3/src/lib.rs', lines 308:16-308:109 -/
+    Source: 'sha3/src/lib.rs', lines 313:16-313:109 -/
 @[reducible]
 def sha512_ema.pre
   (digest : Slice Std.U8) (payload : Slice Std.U8) : RustM Bool := do
@@ -210,7 +226,7 @@ def sha512_ema.pre
   else ok false
 
 /-- [libcrux_iot_sha3::sha512_ema::post]:
-    Source: 'sha3/src/lib.rs', lines 312:0-312:84 -/
+    Source: 'sha3/src/lib.rs', lines 317:0-317:84 -/
 @[reducible]
 def sha512_ema.post
   (digest : Slice Std.U8) (payload : Slice Std.U8)
@@ -228,7 +244,7 @@ def sha512_ema.spec (digest : Slice Std.U8) (payload : Slice Std.U8) : Prop :=
 
 
 /-- [libcrux_iot_sha3::shake128::pre]:
-    Source: 'sha3/src/lib.rs', lines 326:16-326:61 -/
+    Source: 'sha3/src/lib.rs', lines 331:16-331:61 -/
 @[reducible]
 def shake128.pre (BYTES : Std.Usize) (data : Slice Std.U8) : RustM Bool := do
   let i ← lift (UScalar.cast .Usize core.num.U32.MAX)
@@ -242,7 +258,7 @@ def shake128.spec (BYTES : Std.Usize) (data : Slice Std.U8) : Prop :=
 
 
 /-- [libcrux_iot_sha3::shake128_ema::pre]:
-    Source: 'sha3/src/lib.rs', lines 346:16-346:65 -/
+    Source: 'sha3/src/lib.rs', lines 351:16-351:65 -/
 @[reducible]
 def shake128_ema.pre
   (out : Slice Std.U8) (data : Slice Std.U8) : RustM Bool := do
@@ -258,7 +274,7 @@ def shake128_ema.spec (out : Slice Std.U8) (data : Slice Std.U8) : Prop :=
 
 
 /-- [libcrux_iot_sha3::shake256::pre]:
-    Source: 'sha3/src/lib.rs', lines 355:16-355:61 -/
+    Source: 'sha3/src/lib.rs', lines 360:16-360:61 -/
 @[reducible]
 def shake256.pre (BYTES : Std.Usize) (data : Slice Std.U8) : RustM Bool := do
   let i ← lift (UScalar.cast .Usize core.num.U32.MAX)
@@ -272,7 +288,7 @@ def shake256.spec (BYTES : Std.Usize) (data : Slice Std.U8) : Prop :=
 
 
 /-- [libcrux_iot_sha3::shake256_ema::pre]:
-    Source: 'sha3/src/lib.rs', lines 375:16-375:65 -/
+    Source: 'sha3/src/lib.rs', lines 380:16-380:65 -/
 @[reducible]
 def shake256_ema.pre
   (out : Slice Std.U8) (data : Slice Std.U8) : RustM Bool := do
@@ -288,7 +304,7 @@ def shake256_ema.spec (out : Slice Std.U8) (data : Slice Std.U8) : Prop :=
 
 
 /-- [libcrux_iot_sha3::keccakx1::pre]:
-    Source: 'sha3/src/lib.rs', lines 587:16-589:1 -/
+    Source: 'sha3/src/lib.rs', lines 592:16-594:1 -/
 @[reducible]
 def keccakx1.pre
   (RATE : Std.Usize) (DELIM : Std.U8) (data : Slice Std.U8)
@@ -1162,7 +1178,7 @@ def state.KeccakState.set_lane.spec (self : state.KeccakState) (i : Std.Usize)
 
 
 /-- [libcrux_iot_sha3::incremental::{impl libcrux_iot_sha3::incremental::Xof<168usize> for libcrux_iot_sha3::incremental::Shake128Xof}::absorb::pre]:
-    Source: 'sha3/src/lib.rs', lines 461:20-461:39 -/
+    Source: 'sha3/src/lib.rs', lines 466:20-466:39 -/
 @[reducible]
 def incremental.XofShake128Xof168.absorb.pre
   (self_ : incremental.Shake128Xof) (input : Slice Std.U8) : RustM Bool := do
@@ -1187,7 +1203,7 @@ def incremental.Shake128Xof.Insts.Libcrux_iot_sha3IncrementalXof168.absorb.spec
 
 
 /-- [libcrux_iot_sha3::incremental::{impl libcrux_iot_sha3::incremental::Xof<168usize> for libcrux_iot_sha3::incremental::Shake128Xof}::absorb_final::pre]:
-    Source: 'sha3/src/lib.rs', lines 461:20-461:39 -/
+    Source: 'sha3/src/lib.rs', lines 466:20-466:39 -/
 @[reducible]
 def incremental.XofShake128Xof168.absorb_final.pre
   (self_ : incremental.Shake128Xof) (input : Slice Std.U8) : RustM Bool := do
@@ -1213,7 +1229,7 @@ def
 
 
 /-- [libcrux_iot_sha3::incremental::{impl libcrux_iot_sha3::incremental::Xof<136usize> for libcrux_iot_sha3::incremental::Shake256Xof}::absorb::pre]:
-    Source: 'sha3/src/lib.rs', lines 489:20-489:39 -/
+    Source: 'sha3/src/lib.rs', lines 494:20-494:39 -/
 @[reducible]
 def incremental.XofShake256Xof136.absorb.pre
   (self_ : incremental.Shake256Xof) (input : Slice Std.U8) : RustM Bool := do
@@ -1238,7 +1254,7 @@ def incremental.Shake256Xof.Insts.Libcrux_iot_sha3IncrementalXof136.absorb.spec
 
 
 /-- [libcrux_iot_sha3::incremental::{impl libcrux_iot_sha3::incremental::Xof<136usize> for libcrux_iot_sha3::incremental::Shake256Xof}::absorb_final::pre]:
-    Source: 'sha3/src/lib.rs', lines 489:20-489:39 -/
+    Source: 'sha3/src/lib.rs', lines 494:20-494:39 -/
 @[reducible]
 def incremental.XofShake256Xof136.absorb_final.pre
   (self_ : incremental.Shake256Xof) (input : Slice Std.U8) : RustM Bool := do
