libcrux-iot/sha3/proofs/lean/LibcruxIotSha3/Extraction/Types.lean
@@ -72,7 +72,7 @@ def keccak.keccak.closure_1 (RATE : Std.Usize) (DELIM : Std.U8) :=
 def keccak.keccak.closure (RATE : Std.Usize) (DELIM : Std.U8) := Std.Usize
 
 /-- [libcrux_iot_sha3::Algorithm]
-    Source: 'sha3/src/lib.rs', lines 87:0-99:1
+    Source: 'sha3/src/lib.rs', lines 92:0-104:1
     Visibility: public -/
 @[discriminant u32 [1,2,3,4]]
 inductive Algorithm where
@@ -82,24 +82,24 @@ inductive Algorithm where
 | Sha512 : Algorithm
 
 /-- Trait declaration: [libcrux_iot_sha3::incremental::private::Sealed]
-    Source: 'sha3/src/lib.rs', lines 401:8-401:27
+    Source: 'sha3/src/lib.rs', lines 406:8-406:27
     Visibility: public -/
 structure incremental.private.Sealed (Self : Type) where
 
 /-- [libcrux_iot_sha3::incremental::Shake128Xof]
-    Source: 'sha3/src/lib.rs', lines 408:4-410:5
+    Source: 'sha3/src/lib.rs', lines 413:4-415:5
     Visibility: public -/
 structure incremental.Shake128Xof where
   state : keccak.KeccakXofState 168#usize
 
 /-- [libcrux_iot_sha3::incremental::Shake256Xof]
-    Source: 'sha3/src/lib.rs', lines 413:4-415:5
+    Source: 'sha3/src/lib.rs', lines 418:4-420:5
     Visibility: public -/
 structure incremental.Shake256Xof where
   state : keccak.KeccakXofState 136#usize
 
 /-- Trait declaration: [libcrux_iot_sha3::incremental::Xof]
-    Source: 'sha3/src/lib.rs', lines 420:4-459:5
+    Source: 'sha3/src/lib.rs', lines 425:4-464:5
     Visibility: public -/
 structure incremental.Xof (Self : Type) (RATE : Std.Usize) where
   privateSealedInst : incremental.private.Sealed Self
